refactor smallstep

KLR/Semantics/Logic.lean
@@ -9,62 +9,116 @@ import Iris.Algebra.OFE
 import Iris.Algebra.UPred
 import Iris.Instances.UPred
 import Iris.Instances.heProp
+import Iris.BI.BI
 
 -- The logic: I can reuse UPred with a fixed ghost state (first-order)
 -- I'll want the fixpoint combinator to define the wp
 -- Need to port some more of the upred rules most likely
 
 section weakestpre
+open Iris.BI.BIBase
 
 variable {DataT : Type _}
 
 
+abbrev prog := (NML.NMLSemantics DataT).prog
+abbrev state := (NML.NMLSemantics DataT).state
+abbrev val := (NML.NMLSemantics DataT).val
+abbrev step := (NML.NMLSemantics DataT).step
+abbrev to_val := (NML.NMLSemantics DataT).to_val
 
+abbrev PNat := { n : Nat // 0 < n }
 
+instance : DFractional PNat where
+  proper n := n.1 = 1
+  add := sorry
+  add_comm := sorry
+  add_assoc := sorry
+  add_left_cancel := sorry
+  add_ne := sorry
+  proper_add_mono_left := sorry
+  one := sorry
+  whole_iff_one := sorry
 
+structure ProdChipMemory (T : Type _) where
+  left : KLR.Core.ChipMemory T
+  right : KLR.Core.ChipMemory T
+
+inductive ProdIndex
+| left (_ : KLR.Core.DualMemoryStoreIndex)
+| right (_ : KLR.Core.DualMemoryStoreIndex)
+
+instance {T : Type _} : Heap (ProdChipMemory T) ProdIndex T where
+  get := sorry
+  set := sorry
+  of_fun := sorry
+  fresh := sorry
+  get_set_eq := sorry
+  get_set_ne := sorry
+  of_fun_get := sorry
+  point := sorry
+  fresh_get := sorry
+  point_get_eq := sorry
+  point_get_ne := sorry
+
+def TProd (H : Type _ → Type _) (T : Type _) : Type _ := H T × H T
+
+abbrev PROP : Type _ := heProp PNat ProdIndex UInt8 ProdChipMemory
+
+-- The state interpretation, ie the global version of the program state.
+def state_interp (l r : @state DataT) : PROP :=
+  heProp_auth _ _ _ _ (.mk l.memory r.memory)
+  -- Strong relational invariant goes here?
+
+def wp_F (wp : @prog DataT → @prog DataT → (@val DataT → @val DataT→ PROP) → PROP)
+         (p1 p2 : @prog DataT)
+         (Φf : @val DataT → @val DataT → PROP) : PROP :=
+  -- For any pair of states that satisfy the state interpretation...
+  «forall» fun sl : @state DataT =>
+  «forall» fun sr : @state DataT =>
+    iprop(state_interp sl sr -∗
+      -- Either, that configuration is a value, and the postcondition holds,
+      (|==>
+        «exists» fun vl : @val DataT =>
+        «exists» fun vr : @val DataT =>
+        iprop(⌜to_val (p1, sl) = some vl⌝ ∗ ⌜to_val (p2, sr) = some vr⌝ ∗ Φf vl vr)) ∨
+      -- Or, for any two configurations that we can step into, in some number of steps,
+      ( «forall» fun cl' : @prog DataT × @state DataT =>
+        «forall» fun cr' : @prog DataT × @state DataT =>
+        «exists» fun nl : Nat =>
+        «exists» fun nr : Nat =>
+        iprop(
+          ⌜(NML.NMLSemantics DataT).stepN nl.succ (p1, sl) cl' ∧
+            (NML.NMLSemantics DataT).stepN nr.succ (p2, sr) cr'⌝ -∗
+            -- We can reobtain the state interp for the new state, and also
+            -- prove the weakest precondition.
+            ▷ |==> (state_interp cl'.2 cr'.2 ∗ wp cl'.1 cr'.1 Φf))))
+
+instance : Iris.OFE.Contractive (α := @prog DataT → @prog DataT → (@val DataT → @val DataT → PROP) → PROP) wp_F := by
+  sorry
+
+/-- Definition of the weakest precondition -/
+def wp (p1 p2 : @prog DataT) (Φf : @val DataT → @val DataT → PROP) : PROP :=
+  (Iris.fixpoint wp_F) p1 p2 Φf
 
 end weakestpre
 
+-- TODO: I really do want values to only be dependent on the expression.
+-- Stuckness can still depend on the state (I think that's what I wanted anyways?) but
+-- generalizing to values in the cfg is very hard.
+-- To get the specs I want (ie. about the final state) I'll need a more souped up adequacy theorem.
+-- Namely, I'll want an adequacy theorem that can also talk about the memory in the strong relational
+-- invariant.
+theorem wp_value_value_fupd {pl pr : @prog DataT} (Φf : @val DataT → @val DataT → PROP) :
+  (⊢ wp pl pr Φf) → ⊢ (True : PROP)
+  := sorry
 
 
-/-
 
-section logic_test
-open Iris NML Iris.BI.BIBase Lean
 
-variable {Heap : Type _} [UCMRA Heap] {DataT : Type _}
-
-abbrev PROP := UPred Heap
-
--- Agreement over the NKI heaps
--- TODO:
-def state_interp : State × State → UPred Heap := sorry
-
--- The relation that defines the product steps we can take
-def PREL : Cfg × Cfg → (Cfg × Cfg → UPred Heap) → UPred Heap :=
-  sorry
-
--- A standard Iris WP
--- Note: Iris-lean → is Iris -d> by default
--- TODO: Lift to products
-def wp_F (wp : Pgm × Pgm → (@Value DataT × @Value DataT → UPred Heap) → UPred Heap)
-    (p : Pgm × Pgm) (Φ : @Value DataT × @Value DataT → UPred Heap) : UPred Heap :=
-  «forall» fun sl : State =>
-  «forall» fun sr : State =>
-  -- TODO: Merge update syntax into iris-lean main brainc
-  iprop(state_interp (sl, sr) -∗ PREL ((p.1, sl), (p.2, sr))
-    (fun ((pl', sl'), (pr', sr')) => iprop(▷ (state_interp (sl', sr') ∗ wp (pl', pr') Φ))))
-
-def wp (p : Pgm × Pgm) (Φ : @Value DataT × @Value DataT → UPred Heap) : UPred Heap :=
-  -- Port: The fixpoint theorem we skipped to close over wp_F
-  sorry
-
-def triple (pre : UPred Heap) (p1 p2 : Pgm) (post : @Value DataT × @Value DataT → UPred Heap) :=
-  iprop(pre -∗ wp (p1, p2) post)
+/-- Definition for Hoare Triple -/
+def triple (pre : PROP) (p1 p2 : @prog DataT) (post : @val DataT → @val DataT → PROP) :=
+  iprop(pre -∗ wp p1 p2 post)
 
 macro "{{ " pre:term  " }} " p1:term " × " p2:term "{{ " x:ident  " => " post:term " }} " : term => do
   ``(triple $pre $p1 $p2 (fun $x => $post))
-
-end logic_test
-
--/
